Add predicates for tree properties in ArrayTreeUtils: IsCompact, IsSorted, and IsArrayTree. Update Add method to use comparison function for empty checks.

ArrayTreeUtils.dfy
@@ -1,14 +1,66 @@
 module {:extern "ArrayTreeUtils"} ArrayTreeUtils
 {
 	function Left(i: nat): nat { 2 * i + 1 }
+
 	function Right(i: nat): nat { Left(i) + 1 }
+
+	// Predicate to check if the subtree rooted at index is compact
+	predicate IsCompact<T(!new)(==)(0)>(x: array<T>, empty: T, compare: (T, T) -> int, index: nat)
+		reads x
+		requires 0 <= index < x.Length
+		decreases x.Length - index
+	{
+		if compare(x[index], empty) == 0 then
+			if Right(index) < x.Length then
+				IsCompact(x, empty, compare, Left(index)) && IsCompact(x, empty, compare, Right(index))
+			else
+				true
+		else
+			false
+	}
+
+	predicate LessIfNotEmpty<T(!new)(==)(0)>(a : T, b: T, empty: T, compare: (T, T) -> int)
+	{
+		if compare(a, empty) == 0 || compare(b, empty) == 0 then
+			true
+		else
+			compare(a, b) < 0
+	}
+
+	predicate IsSorted<T(!new)(==)(0)>(x: array<T>, empty: T, compare: (T, T) -> int, index: nat)
+		reads x
+		requires 0 <= index < x.Length
+		decreases x.Length - index
+	{
+		if compare(x[index], empty) == 0 then
+			true
+		else
+			if Right(index) < x.Length then
+				LessIfNotEmpty(x[Left(index)], x[Right(index)], empty, compare) &&
+				LessIfNotEmpty(x[Left(index)], x[index], empty, compare) &&
+				LessIfNotEmpty(x[index], x[Right(index)], empty, compare) &&
+				IsSorted(x, empty, compare, Left(index)) &&
+				IsSorted(x, empty, compare, Right(index))
+			else
+				true
+	}
+
+	predicate IsArrayTree<T(!new)(==)(0)>(x: array<T>, empty: T, compare: (T, T) -> int)
+		reads x
+		requires 0 < x.Length
+		decreases x.Length
+	{
+		IsCompact(x, empty, compare, 0) &&
+		IsSorted(x, empty, compare, 0)
+	}
 
 	method Add<T(!new)(==)(0)>(x: array<T>, item: T, empty: T, compare: (T, T) -> int)
 		returns (position: nat)
 		modifies x
+		requires 0 < x.Length && IsArrayTree(x, empty, compare)
 	{
 		var index := 0;
-		while index < x.Length && x[index] != empty
+		while index < x.Length && compare(x[index], empty) != 0
 		{
 			if compare(item, x[index]) == 0
 			{
@@ -35,7 +87,7 @@ module {:extern "ArrayTreeUtils"} ArrayTreeUtils
 		ensures position != -1 ==> 0 <= position < x.Length && compare(item, x[position]) == 0
 	{
 		var index := 0;
-		while index < x.Length && x[index] != empty
+		while index < x.Length && compare(x[index], empty) != 0
 			invariant index >= 0
 		{
 			if compare(item, x[index]) == 0
